coq/simple-instance/TraceSemantics.v
@@ -42,14 +42,23 @@ Definition dual (t:trace) :=
                   STATES
    _____________________________________ *)
 
+Inductive slash : Type := Slash.
+
+Definition sigma :=
+  call_stack.
+
 Definition A_sigma :=
-  list component_id.
+  list (component_id * slash).
+
+Inductive alt_list (a b: Type): Type :=
+  | init : a -> alt_list a b
+  | cons : a -> alt_list b a -> alt_list a b.
+
+Definition A_SIGMA : Type :=
+  alt_list A_sigma sigma.
 
 Definition P_SIGMA : Type :=
-  admit.
-
-Definition A_SIGMA : Type := 
-  admit.
+  alt_list sigma A_sigma.
 
 Definition program_state : Type :=
   (component_id *
@@ -70,8 +79,41 @@ Inductive state_partial_view : Type :=
 
 (* ------- Definitions : Extra notations ------- *)
 
-(*Definition Top (PE:P_SIGMA) :=
-  match PE with
-  |  
-*)
+Definition Top_PSIGMA (PE:P_SIGMA) : sigma :=
+  admit.
+
+Definition Top_ASIGMA (AE:A_SIGMA) : sigma :=
+  admit.
+
+Definition SetTop_PSIGMA (PE:P_SIGMA) (o:sigma) : P_SIGMA :=
+  admit.
+
+Definition SetTop_ASIGMA (AE:A_SIGMA) (Ao:A_sigma) : A_SIGMA :=
+  admit.
+
+
+(* _____________________________________ 
+                REDUCTIONS
+   _____________________________________ *)
+
+Inductive reduction (Is:program_interfaces) (E:entry_points) : 
+  program_state -> program_state -> action -> Prop :=
+  | T_CallRetTauPlus :
+    forall C C' d d' mem mem' reg reg' pc pc' o o' PE PE',
+    let action := fun cfg =>
+      match cfg with
+      | (C,d,mem,reg,pc) =>
+        match decode (fetch_mem C mem pc) with
+        | Some (Call C0 P0) => Int (IntCall C0 P0) ProgramOrigin
+        | Some Return => Int IntRet ProgramOrigin 
+        | _ => Int IntTau ProgramOrigin
+        end
+      end
+    in 
+    Top_PSIGMA = o -> PE' = SetTop_PSIGMA PE o' ->
+    step Is E (C,d,mem,reg,pc) (C',d',mem',reg',pc') ->
+    reduction Is E (C,PE,mem,reg,pc) (C',PE',mem',reg',pc')
+    (action (C,d,mem,reg,pc)). 
+
+
 
